src/Init/Data/Nat/Control.lean
@@ -11,44 +11,44 @@ import Init.Omega
 namespace Nat
 universe u v
 
-@[inline] def forM {m} [Monad m] (n : Nat) (f : Fin n → m Unit) : m Unit :=
+@[inline] def forM {m} [Monad m] (n : Nat) (f : (i : Nat) → i < n → m Unit) : m Unit :=
   let rec @[specialize] loop : ∀ i, i ≤ n → m Unit
     | 0,   _ => pure ()
-    | i+1, h => do f ⟨n-i-1, by omega⟩; loop i (Nat.le_of_succ_le h)
+    | i+1, h => do f (n-i-1) (by omega); loop i (Nat.le_of_succ_le h)
   loop n (by simp)
 
-@[inline] def forRevM {m} [Monad m] (n : Nat) (f : Fin n → m Unit) : m Unit :=
+@[inline] def forRevM {m} [Monad m] (n : Nat) (f : (i : Nat) → i < n → m Unit) : m Unit :=
   let rec @[specialize] loop : ∀ i, i ≤ n → m Unit
     | 0,   _ => pure ()
-    | i+1, h => do f ⟨i, by omega⟩; loop i (Nat.le_of_succ_le h)
+    | i+1, h => do f i (by omega); loop i (Nat.le_of_succ_le h)
   loop n (by simp)
 
-@[inline] def foldM {α : Type u} {m : Type u → Type v} [Monad m] (n : Nat) (f : Fin n → α → m α) (init : α) : m α :=
+@[inline] def foldM {α : Type u} {m : Type u → Type v} [Monad m] (n : Nat) (f : (i : Nat) → i < n → α → m α) (init : α) : m α :=
   let rec @[specialize] loop : ∀ i, i ≤ n → α → m α
     | 0,   h, a => pure a
-    | i+1, h, a => f ⟨n-i-1, by omega⟩ a >>= loop i (by omega)
+    | i+1, h, a => f (n-i-1) (by omega) a >>= loop i (Nat.le_of_succ_le h)
   loop n (by omega) init
 
-@[inline] def foldRevM {α : Type u} {m : Type u → Type v} [Monad m] (n : Nat) (f : Fin n → α → m α) (init : α) : m α :=
+@[inline] def foldRevM {α : Type u} {m : Type u → Type v} [Monad m] (n : Nat) (f : (i : Nat) → i < n → α → m α) (init : α) : m α :=
   let rec @[specialize] loop : ∀ i, i ≤ n → α → m α
     | 0,   h, a => pure a
-    | i+1, h, a => f ⟨i, by omega⟩ a >>= loop i (by omega)
+    | i+1, h, a => f i (by omega) a >>= loop i (Nat.le_of_succ_le h)
   loop n (by omega) init
 
-@[inline] def allM {m} [Monad m] (n : Nat) (p : Fin n → m Bool) : m Bool :=
+@[inline] def allM {m} [Monad m] (n : Nat) (p : (i : Nat) → i < n → m Bool) : m Bool :=
   let rec @[specialize] loop : ∀ i, i ≤ n → m Bool
     | 0,   _ => pure true
     | i+1 , h => do
-      match (← p ⟨n-i-1, by omega⟩) with
+      match (← p (n-i-1) (by omega)) with
       | true  => loop i (by omega)
       | false => pure false
   loop n (by simp)
 
-@[inline] def anyM {m} [Monad m] (n : Nat) (p : Fin n → m Bool) : m Bool :=
+@[inline] def anyM {m} [Monad m] (n : Nat) (p : (i : Nat) → i < n → m Bool) : m Bool :=
   let rec @[specialize] loop : ∀ i, i ≤ n → m Bool
     | 0,   _ => pure false
     | i+1, h => do
-      match (← p ⟨n-i-1, by omega⟩) with
+      match (← p (n-i-1) (by omega)) with
       | true  => pure true
       | false => loop i (Nat.le_of_succ_le h)
   loop n (by simp)
