src/Lean/Compiler/IR/Borrow.lean
@@ -205,7 +205,7 @@ def getParamInfo (k : ParamMap.Key) : M (Array Param) := do
 
 /-- For each ps[i], if ps[i] is owned, then mark xs[i] as owned. -/
 def ownArgsUsingParams (xs : Array Arg) (ps : Array Param) : M Unit :=
-  xs.size.forM fun i => do
+  xs.size.forM fun i _ => do
     let x := xs[i]
     let p := ps[i]!
     unless p.borrow do ownArg x
@@ -216,7 +216,7 @@ def ownArgsUsingParams (xs : Array Arg) (ps : Array Param) : M Unit :=
    we would have to insert a `dec xs[i]` after `f xs` and consequently
    "break" the tail call. -/
 def ownParamsUsingArgs (xs : Array Arg) (ps : Array Param) : M Unit :=
-  xs.size.forM fun i => do
+  xs.size.forM fun i _ => do
     let x := xs[i]
     let p := ps[i]!
     match x with
