src/Lean/Compiler/IR/ElimDeadBranches.lean
@@ -225,7 +225,7 @@ def updateCurrFnSummary (v : Value) : M Unit := do
 def updateJPParamsAssignment (ys : Array Param) (xs : Array Arg) : M Bool := do
   let ctx ← read
   let currFnIdx := ctx.currFnIdx
-  ys.size.foldM (init := false) fun i r => do
+  ys.size.foldM (init := false) fun i _ r => do
     let y := ys[i]
     let x := xs[i]!
     let yVal ← findVarValue y.x
@@ -282,7 +282,7 @@ partial def interpFnBody : FnBody → M Unit
 def inferStep : M Bool := do
   let ctx ← read
   modify fun s => { s with assignments := ctx.decls.map fun _ => {} }
-  ctx.decls.size.foldM (init := false) fun idx modified => do
+  ctx.decls.size.foldM (init := false) fun idx _ modified => do
     match ctx.decls[idx] with
     | .fdecl (xs := ys) (body := b) .. => do
       let s ← get
