src/Lean/Compiler/IR/ExpandResetReuse.lean
@@ -134,7 +134,7 @@ abbrev M := ReaderT Context (StateM Nat)
   modifyGet fun n => ({ idx := n }, n + 1)
 
 def releaseUnreadFields (y : VarId) (mask : Mask) (b : FnBody) : M FnBody :=
-  mask.size.foldM (init := b) fun i b =>
+  mask.size.foldM (init := b) fun i _ b =>
     match mask[i] with
     | some _ => pure b -- code took ownership of this field
     | none   => do
