src/Lean/Data/PersistentArray.lean
@@ -4,6 +4,7 @@ Released under Apache 2.0 license as described in the file LICENSE.
 Authors: Leonardo de Moura
 -/
 prelude
+import Init.Data.Nat.Fold
 import Init.Data.Array.Basic
 import Init.NotationExtra
 import Init.Data.ToString.Macro
