src/Lean/Meta/Tactic/Induction.lean
@@ -134,9 +134,9 @@ def getMajorTypeIndices (mvarId : MVarId) (tacticName : Name) (recursorInfo : Re
     if idxPos ≥ majorTypeArgs.size then throwTacticEx tacticName mvarId m!"major premise type is ill-formed{indentExpr majorType}"
     let idx := majorTypeArgs.get! idxPos
     unless idx.isFVar do throwTacticEx tacticName mvarId m!"major premise type index {idx} is not a variable{indentExpr majorType}"
-    majorTypeArgs.size.forM fun i => do
+    majorTypeArgs.size.forM fun i _ => do
       let arg := majorTypeArgs[i]
-      if i.1 != idxPos && arg == idx then
+      if i != idxPos && arg == idx then
         throwTacticEx tacticName mvarId m!"'{idx}' is an index in major premise, but it occurs more than once{indentExpr majorType}"
       if i < idxPos then
         if (← exprDependsOn arg idx.fvarId!) then
@@ -146,7 +146,7 @@ def getMajorTypeIndices (mvarId : MVarId) (tacticName : Name) (recursorInfo : Re
       if i > idxPos && recursorInfo.indicesPos.contains i && arg.isFVar then
         let idxDecl ← idx.fvarId!.getDecl
         if (← localDeclDependsOn idxDecl arg.fvarId!) then
-          throwTacticEx tacticName mvarId m!"'{idx}' is an index in major premise, but it depends on index occurring at position #{i.1+1}"
+          throwTacticEx tacticName mvarId m!"'{idx}' is an index in major premise, but it depends on index occurring at position #{i+1}"
     return idx
 
 /--
